updates

Veritas.SeqAux.fst
@@ -2,6 +2,7 @@ module Veritas.SeqAux
 
 open FStar.Classical
 open FStar.Seq
+open FStar.Squash
 
 let prefix (#a:Type) (s:seq a) (i:nat{i <= length s}) = slice s 0 i
 
@@ -12,12 +13,12 @@ let lemma_prefix_index (#a:Type) (s:seq a) (i:nat{i <= length s}) (j:nat{j < i})
 
 let lemma_prefix_prefix (#a:Type) (s:seq a) (i:nat{i <= length s}) (j:nat{j <= i}):
   Lemma (requires (True))
-        (ensures (prefix (prefix s i) j == prefix s j)) = 
+        (ensures (prefix (prefix s i) j == prefix s j)) =
   let pij = prefix (prefix s i) j in
   let pj = prefix s j in
   let pi = prefix s i in
   let aux (k:nat{k < j}):
-    Lemma (index pij k == index pj k) = 
+    Lemma (index pij k == index pj k) =
     lemma_prefix_index s j k;
     lemma_prefix_index s i k;
     lemma_prefix_index pi j k
@@ -26,14 +27,20 @@ let lemma_prefix_prefix (#a:Type) (s:seq a) (i:nat{i <= length s}) (j:nat{j <= i
 
 let lemma_fullprefix_equal (#a:Type) (s:seq a):
   Lemma (requires (True))
-        (ensures (prefix s (length s) == s)) = 
+        (ensures (prefix s (length s) == s)) =
   let n = length s in
   let p = prefix s n in
   let aux (k:nat{k < n}):
-    Lemma (index p k == index s k) = 
+    Lemma (index p k == index s k) =
     lemma_prefix_index s n k
   in
   forall_intro aux; lemma_eq_intro s p
+
+let lemma_prefix_append (#a:Type) (s1 s2: seq a):
+  Lemma (prefix (append s1 s2) (length s1) == s1) =
+  // triggers an SMT pat that provides what we need
+  assert(equal (prefix (append s1 s2) (length s1)) s1);
+  ()
 
 let suffix (#a:Type) (s:seq a) (i:nat{i <= length s}) =
   slice s (length s - i) (length s)
@@ -43,22 +50,219 @@ let lemma_suffix_index (#a:Type) (s:seq a) (i:nat{i <= length s}) (j:nat{j < i})
         (ensures (index (suffix s i) j == index s (length s - i + j))) =
   lemma_index_slice s (length s - i) (length s) j
 
-(*
- * TODO: For some reason a direct recursive implementation of filter
- * fails to compile
- *)
-let rec filter_aux (#a:eqtype) (f:a -> bool) (s:seq a) : Tot (seq (refine f))
+let lemma_prefix_suffix (#a:Type) (s:seq a) (i:nat{i <= length s}):
+  Lemma (requires (True))
+        (ensures (append (prefix s i) (suffix s (length s - i)) == s)) =
+  assert(equal (append (prefix s i) (suffix s (length s - i))) s);
+  ()
+
+(* append a single element to the end of a sequence *)
+let append1 (#a:eqtype) (s:seq a) (x:a): s':(seq a){length s' = length s + 1} =
+  append s (create 1 x)
+
+type proj (#a:eqtype): seq a -> seq a -> Type0 =
+  | PrjEmpty: proj (empty #a) (empty #a)
+  | PrjIncl: ss: seq a -> s:seq a -> prf:proj ss s -> x:a -> proj (append1 ss x) (append1 s x)
+  | PrjSkip: ss: seq a -> s:seq a -> prf:proj ss s -> x:a -> proj ss (append1 s x)
+
+let rec proj_index_map_aux (#a:eqtype) (ss: seq a) (s: seq a) (prf:proj ss s) (i:seq_index ss) :
+  Tot (j:seq_index s{index s j = index ss i})
+  (decreases (length s))
+  =
+  let n = length s in
+  let ns = length ss in
+  match prf with
+  | PrjIncl ss' s' prf' e ->
+    if i = ns - 1 then
+      n - 1
+    else
+      proj_index_map_aux ss' s' prf' i
+  | PrjSkip ss' s' prf' x -> proj_index_map_aux ss' s' prf' i
+
+let proj_index_map (#a:eqtype) (ss s: seq a) (prf: proj ss s) (i: seq_index ss) = 
+  proj_index_map_aux ss s prf i
+
+(* the mapping we construct above is monotonic *)
+let rec lemma_proj_monotonic_aux (#a:eqtype) (ss s: seq a) (prf: proj ss s) (i1 i2: seq_index ss):
+  Lemma (requires (i1 < i2))
+        (ensures (proj_index_map ss s prf i1 < proj_index_map ss s prf i2)) 
+        (decreases prf) = 
+  match prf with
+  | PrjIncl ss' s' prf' _ -> 
+    if i2 = length ss - 1 then ()
+    else lemma_proj_monotonic_aux ss' s' prf' i1 i2
+  | PrjSkip ss' s' prf' _ -> lemma_proj_monotonic_aux ss' s' prf' i1 i2
+
+let lemma_proj_monotonic (#a:eqtype) (ss s: seq a) (prf: proj ss s) (i1 i2: seq_index ss):
+  Lemma (requires (i1 < i2))
+        (ensures (proj_index_map ss s prf i1 < proj_index_map ss s prf i2)) = 
+  lemma_proj_monotonic_aux ss s prf i1 i2
+
+let rec lemma_proj_length_aux (#a:eqtype) (ss s: seq a) (prf: proj ss s): 
+  Lemma (requires (True)) 
+        (ensures (length ss <= length s))
+        (decreases prf) = 
+  match prf with
+  | PrjEmpty -> ()
+  | PrjIncl ss' s' prf' _ -> lemma_proj_length_aux ss' s' prf'
+  | PrjSkip ss' s' prf' _ -> lemma_proj_length_aux ss' s' prf'
+
+let lemma_as_squash #a #b (lem: (a -> Lemma b)) (x:a)
+  : GTot (squash b)
+  = lem x
+
+let lemma_proj_length (#a:eqtype) (ss: seq a) (s:seq a{proj ss s}):
+  Lemma (requires (True))
+        (ensures (length ss <= length s)) = 
+  bind_squash () (lemma_as_squash #(proj ss s) #(length ss <= length s) (lemma_proj_length_aux ss s))
+
+let rec filter_aux (#a:eqtype) (f:a -> bool) (s:seq a) : Tot (seq a)
   (decreases (length s)) =
   let n = length s in
   if n = 0 then empty
   else
     let e = index s (n - 1) in
     if f e then
-      append (filter_aux f (prefix s (n - 1))) (create 1 e)
+      append1 (filter_aux f (prefix s (n - 1))) e
     else
       filter_aux f (prefix s (n - 1))
 
-let filter (#a:eqtype) (f:a -> bool) (s:seq a) : Tot (seq (refine f))  = filter_aux f s
+let filter (#a:eqtype) (f:a -> bool) (s:seq a) : Tot (seq a)  = filter_aux f s
+
+let rec filter_is_proj_aux (#a:eqtype) (f:a -> bool) (s:seq a): Tot (proj (filter f s) s)
+  (decreases (length s)) =
+  let n = length s in
+  let fs = filter f s in
+  if n = 0 then (
+    lemma_empty s;
+    PrjEmpty #a
+  )
+  else (
+
+    let e = index s (n - 1) in
+    let s' = prefix s (n - 1) in
+    let fs' = filter f s' in
+    assert (equal (append1 s' e) s);
+    let prf = filter_is_proj_aux f s' in
+    if f e then
+      PrjIncl fs' s' prf e
+    else
+      PrjSkip fs' s' prf e
+  )
+
+let lemma_filter_is_proj (#a:eqtype) (f:a -> bool) (s:seq a):
+  Lemma (proj (filter f s) s) = return_squash (filter_is_proj_aux f s)
+
+let filter_is_proj_prf (#a:eqtype) (f:a -> bool) (s: seq a) = filter_is_proj_aux f s
+
+(* every index in the filtered sequence satisfies the filter predicate *)
+let rec lemma_filter_correct1_aux (#a: eqtype) (f:a -> bool) (s:seq a) (i:seq_index (filter f s)):
+  Lemma (requires (True))
+        (ensures (f (index (filter f s) i) = true))
+        (decreases (length s)) = 
+  let n = length s in
+  let fs = filter f s in
+  if n = 0 then ()
+  else 
+    let s' = prefix s (n - 1) in
+    let e = index s (n - 1) in
+    if f e then
+      if i = (length fs) - 1 then ()
+      else
+        lemma_filter_correct1_aux f s' i
+    else
+      lemma_filter_correct1_aux f s' i
+
+let lemma_filter_correct1 (#a: eqtype) (f:a -> bool) (s:seq a) (i:seq_index (filter f s)):
+  Lemma (requires (True))
+        (ensures (f (index (filter f s) i) = true)) = lemma_filter_correct1_aux f s i
+        
+
+
+(*
+
+let rec projection_aux (#a:eqtype) (ss s: seq a): Tot bool (decreases (length s)) =
+  let nss = length ss in
+  let ns = length s in
+  if nss = 0 then true
+  else if ns = 0 then false
+  else
+    let es = index s (ns - 1) in
+    let ess = index ss (nss - 1) in
+    if projection_aux ss (prefix s (ns - 1)) then true
+    else if es = ess then projection_aux (prefix ss (nss - 1)) (prefix s (ns - 1))
+    else false
+
+let projection (#a:eqtype) (ss s: seq a) = projection_aux ss s
+
+let rec lemma_filter_is_projection_aux (#a:eqtype) (f:a -> bool) (s:seq a):
+  Lemma (requires (True))
+        (ensures (projection (filter f s) s))
+        (decreases (length s)) =
+  let n = length s in
+  if n = 0 then ()
+  else
+    let e = index s (n - 1) in
+    let s' = prefix s (n - 1) in
+    let fs' = filter f s' in
+    if f e then (
+      lemma_filter_is_projection_aux f s';
+      lemma_prefix_append fs' (create 1 e);
+      ()
+    )
+    else
+      lemma_filter_is_projection_aux f s'
+
+let lemma_filter_is_projection (#a:eqtype) (f:a -> bool) (s:seq a):
+  Lemma (projection (filter f s) s) = lemma_filter_is_projection_aux f s
+
+(* mapping from a subsequence index to the corresponding index in the base sequence *)
+let rec projection_index_map_aux (#a:eqtype) (ss: seq a) (s: seq a{projection ss s}) (i:seq_index ss):
+  Tot (j:seq_index s{index s j = index ss i})
+  (decreases (length s)) =
+  let n = length s in
+  let ns = length ss in
+  if ns = 0 then 0       (* contradiction since i < ns *)
+  else if n = 0 then 0   (* contradiction since (projection ss s) is false *)
+  else
+    let s' = prefix s (n - 1) in
+    let e = index s (n - 1) in
+    let ss' = prefix ss (ns - 1) in
+    let es = index ss (ns - 1) in
+    if projection ss s' then
+      projection_index_map_aux ss s' i
+    else (
+      assert (e = es);
+      if i = ns - 1 then n - 1
+      else projection_index_map_aux ss' s' i
+    )
+
+(* mapping from a subsequence index to the corresponding index in the base sequence *)
+let projection_index_map (#a:eqtype) (ss: seq a) (s: seq a{projection ss s}) (i:seq_index ss):
+  Tot (j:seq_index s{index s j = index ss i}) = projection_index_map_aux ss s i
+
+let lemma_projection_monotonic (#a:eqtype) (ss: seq a) (s:seq a{projection ss s}) (i1 i2: seq_index ss):
+  Lemma (requires (i1 < i2))
+        (ensures (projection_index_map ss s i1 < projection_index_map ss s i2))
+
+
+(* every index in the filtered sequence satisfies the filter predicate
+let rec lemma_filter_correct1_aux (#a:Type) (f:a -> bool) (s:seq a) (i:seq_index (filter f s)):
+  Lemma (requires (True))
+        (ensures (f (index (filter f s) i) = true))
+        (decreases (length s)) =
+  let n = length s in
+  if n = 0 then ()
+  else
+    let e = index s (n-  1) in
+    if f e then
+      admit()
+    else
+      admit()
+
+*)
+
+
 
 let rec filter_len_monotonic (#a:eqtype) (f:a -> bool) (s:seq a) (i:nat{i <= length s}):
   Lemma (requires (True))
@@ -96,7 +300,7 @@ let filter_index_map (#a:eqtype) (f:a -> bool) (s:seq a) (i:seq_index s{f (index
   Tot (j:seq_index (filter f s){index s i = index (filter f s) j}) =
   filter_index_map_correct f s i;
   filter_index_map_aux f s i
-         
+
 let filter_index_map_monotonic (#a:eqtype) (f:a -> bool) (s:seq a)
   (i:seq_index s) (j:seq_index s{j > i}):
   Lemma (requires (f (index s i) && f (index s j)))
@@ -128,7 +332,7 @@ let filter_index_inv_map (#a:eqtype) (f:a -> bool)  (s:seq a) (i:seq_index (filt
 let filter_index_inv_map_monotonic (#a:eqtype) (f:a -> bool) (s: seq a)
   (i:seq_index (filter f s)) (j: seq_index (filter f s) {j > i}):
     Lemma (requires (True))
-          (ensures (filter_index_inv_map f s i < filter_index_inv_map f s j)) = 
+          (ensures (filter_index_inv_map f s i < filter_index_inv_map f s j)) =
   let i' = filter_index_inv_map f s i in
   let j' = filter_index_inv_map f s j in
   if i' < j' then () // nothing to prove
@@ -138,10 +342,10 @@ let filter_index_inv_map_monotonic (#a:eqtype) (f:a -> bool) (s: seq a)
 
 let lemma_filter_maps_correct (#a:eqtype) (f:a -> bool) (s: seq a) (i:seq_index s):
   Lemma (requires (f (index s i)))
-        (ensures (filter_index_inv_map f s (filter_index_map f s i) = i)) = 
+        (ensures (filter_index_inv_map f s (filter_index_map f s i) = i)) =
   let i' = filter_index_map f s i in
   let i2 = filter_index_inv_map f s i' in
-  if i2 < i then 
+  if i2 < i then
     filter_index_map_monotonic f s i2 i
   else if i2 > i then
     filter_index_map_monotonic f s i i2
@@ -194,7 +398,7 @@ let lemma_last_index_prefix (#a:eqtype) (f:a -> bool) (s:seq a) (i:nat{i <= leng
 
 let lemma_not_exists_prefix (#a:eqtype) (f:a -> bool) (s:seq a) (i:nat{i <= length s}):
   Lemma (requires (not (exists_sat_elems f s)))
-        (ensures (not (exists_sat_elems f (prefix s i)))) = 
+        (ensures (not (exists_sat_elems f (prefix s i)))) =
   let s' = prefix s i in
   if exists_sat_elems f s' then (
     let li' = last_index f s' in
@@ -205,11 +409,11 @@ let lemma_not_exists_prefix (#a:eqtype) (f:a -> bool) (s:seq a) (i:nat{i <= leng
 
 let lemma_exists_prefix_implies_exists (#a:eqtype) (f:a -> bool) (s:seq a) (i:nat{i <= length s}):
   Lemma (requires (exists_sat_elems f (prefix s i)))
-        (ensures (exists_sat_elems f s)) = 
+        (ensures (exists_sat_elems f s)) =
   let s' = prefix s i in
   let li = last_index f s' in
   lemma_last_index_correct2 f s li
-  
+
 let lemma_last_index_last_elem_nsat (#a:eqtype) (f:a -> bool) (s:seq a{length s > 0}):
   Lemma (requires (not (f (index s (length s - 1)))))
         (ensures ((exists_sat_elems f s ==> last_index f s < length s - 1) /\
@@ -231,9 +435,9 @@ let first_index (#a:eqtype) (f:a -> bool) (s:seq a{exists_sat_elems f s})
 
 let lemma_first_index_correct1 (#a:eqtype) (f:a -> bool) (s:seq a) (i:seq_index s):
   Lemma (requires (exists_sat_elems f s /\ i < first_index f s))
-        (ensures (not (f (index s i)))) = 
+        (ensures (not (f (index s i)))) =
   let fi = first_index f s in
-  if f (index s i) then 
+  if f (index s i) then
     filter_index_map_monotonic f s i fi
   else ()
 
@@ -246,13 +450,13 @@ let lemma_first_index_correct2 (#a:eqtype) (f:a -> bool) (s:seq a) (i:seq_index 
     lemma_first_index_correct1 f s i
   else ()
 
-let rec map_aux (#a #b:Type) (f:a -> b) (s:seq a): 
-  Tot (s':seq b{length s' = length s}) 
+let rec map_aux (#a #b:Type) (f:a -> b) (s:seq a):
+  Tot (s':seq b{length s' = length s})
   (decreases (length s))
-  = 
+  =
   let n = length s in
   if n = 0 then empty
-  else 
+  else
     let ps = prefix s (n - 1) in
     let e = index s (n - 1) in
     append (map_aux f ps) (create 1 (f e))
@@ -262,7 +466,7 @@ let map (#a #b:Type) (f:a -> b) (s:seq a): Tot (s':seq b{length s' = length s}) 
 let rec lemma_map_index_aux (#a #b: Type) (f:a -> b) (s:seq a) (i:seq_index s):
   Lemma (requires (True))
         (ensures (f (index s i) == index (map f s) i))
-        (decreases (length s)) = 
+        (decreases (length s)) =
   let n = length s in
   if n = 0 then ()
   else if i = n - 1 then ()
@@ -275,5 +479,6 @@ let rec lemma_map_index_aux (#a #b: Type) (f:a -> b) (s:seq a) (i:seq_index s):
 
 let lemma_map_index (#a #b: Type) (f:a -> b) (s:seq a) (i:seq_index s):
   Lemma (requires (True))
-        (ensures (f (index s i) == index (map f s) i)) = 
+        (ensures (f (index s i) == index (map f s) i)) =
   lemma_map_index_aux f s i
+*)
