Veritas.SeqOps.fsti
@@ -1,13 +1,102 @@
 module Veritas.SeqOps
 
+open FStar.List.Tot
 open FStar.Seq
-open Veritas.SeqAux
-
-val flat_length (#a:Type) (ss: seq (seq a)): Tot nat
+//open Veritas.SeqAux
 
 (* append a single element to the end of a sequence *)
 let append1 (#a:eqtype) (s:seq a) (x:a): s':(seq a){length s' = length s + 1} = 
-  append s (create 1 x)
+  Seq.append s (create 1 x)
+
+val interleave (#a:eqtype): seq a -> seq a -> seq a -> Type
+
+(*
+(* interleave s s1 s2 indicates s1 is an interleaving of s1 and s2 *)
+(* TODO: Can we hide this definition from users? *)
+type interleave (#a:eqtype): seq a -> seq a -> seq a -> Type =
+  | IntEmpty: interleave #a (empty #a) (empty #a) (empty #a)
+  | IntLeft: s: seq a -> s1: seq a 
+                      -> s2: seq a 
+                      -> prf: interleave s s1 s2 
+                      -> x:a 
+                      -> interleave (append1 s x) (append1 s1 x) s2
+  | IntRight: s: seq a -> s1: seq a 
+                       -> s2: seq a 
+                       -> prf:interleave s s1 s2 
+                       -> x:a
+                       -> interleave (append1 s x) s1 (append1 s x)
+
+*)
+
+(* interleaving is commutative *)
+val lemma_interleave_comm (#a:eqtype) (s s1 s2: seq a):
+  Lemma (requires (interleave s s1 s2))
+        (ensures (interleave s s2 s1))
+
+let aux (#a:eqtype) (s s1 s2: seq a) (prf: interleave s s1 s2):
+  Lemma (false) = admit()
+
+let lemma_something (#a:eqtype) (s s1: seq a) (s2:seq a{interleave s s1 s2}):
+  Lemma (requires (True))
+        (ensures (false)) = 
+  let s':squash (interleave s s1 s2) = () in 
+  FStar.Squash.bind_squash s' (aux s s1 s2) 
+  
+
+(* map an index of interleaved sequence to an index of source sequence *)
+val interleave_map (#a:eqtype) (s:seq a) (s1 s2: seq a) (prf: interleave s s1 s2) (i:seq_index s):
+  Tot (j: (nat*nat){fst j = 0 /\ snd j < length s1 /\ index s i = index s1 (snd j) \/
+                  fst j = 1 /\ snd j < length s2 /\ index s i = index s2 (snd j)})
+
+(* map an index of left sequence to its index in the interleaved sequence *)
+val interleave_inv_map_left (#a:eqtype) (s s1 s2: seq a) (prf: interleave s s1 s2) (i: seq_index s1):
+  Tot (j: seq_index s{index s j = index s1 i /\ interleave_map s s1 s2 prf j = (0,i)})
+
+(* map an index of left sequence to its index in the interleaved sequence *)
+val interleave_inv_map_right (#a:eqtype) (s s1 s2: seq a) (prf: interleave s s1 s2) (i: seq_index s2):
+  Tot (j: seq_index s{index s j = index s2 i /\ interleave_map s s1 s2 prf j = (1,i)})
+
+val lemma_interleave_map_monotonic_left (#a:eqtype) 
+  (s s1 s2: seq a) (prf:interleave s s1 s2) (i1 i2: seq_index s1):
+  Lemma (requires (i1 < i2))
+        (ensures (interleave_inv_map_left s s1 s2 prf i1 < interleave_inv_map_left s s1 s2 prf i2))
+
+val lemma_interleave_map_monotonic_right (#a:eqtype)
+  (s s1 s2: seq a) (prf:interleave s s1 s2) (i1 i2: seq_index s2):
+  Lemma (requires (i1 < i2))
+        (ensures (interleave_inv_map_right s s1 s2 prf i1 < interleave_inv_map_right s s1 s2 prf i2))
+
+(* generalize interleaving to a list of sequences *)
+type interleave_l (#a:eqtype): seq a -> list (seq a) -> Type = 
+  | IntNil: interleave_l #a (empty #a) []
+  | IntApp: s: seq a -> h: seq a -> ts: seq a -> tl: list (seq a) -> prf1: interleave_l ts tl -> 
+            prf2: interleave s h ts -> interleave_l s (h::tl)
+
+module L = FStar.List.Tot
+
+(* interleaving for sequences *)
+type interleave_s (#a:eqtype) (#p:pos): seq a -> ss:(seq (seq a)){length ss = p} -> Type = 
+  | IntSeq: s:seq a -> l: list (seq a){L.length l = p} -> prf:interleave_l s l -> 
+    interleave_s #a #p s (seq_of_list l)
+
+(* projection of a seq obtained by removing some elements *)
+type project (#a:eqtype): seq a -> seq a -> Type = 
+  | PrjEmpty: project (empty #a) (empty #a)
+  | PrjIncl: s:seq a -> s':seq a -> prf:project s s' -> x:a -> project (append1 s x) (append1 s' x)
+  | PrjSkip: s:seq a -> s':seq a -> prf:project s s' -> x:a -> project (append1 s x) s'
+
+(* projection and interleaving are isomorphic *)
+val lemma_interleave_implies_project (#a:eqtype) (s s1 s2: seq a):
+  Lemma (requires (interleave s s1 s2))
+        (ensures (project s s1))
+
+val project_to_interleave (#a:eqtype) (s s1: seq a) (prf: project s s1): s2:_ {interleave s s1 s2}
+
+
+
+(*
+val flat_length (#a:Type) (ss: seq (seq a)): Tot nat
+
 
 (* append a single element to the i'th seq in a sequence of sequences *)
 let append1seq (#a:eqtype)
@@ -26,8 +115,6 @@ type interleave (#a:eqtype) (#p:pos): seq a -> ss:(seq (seq a)){length ss = p} -
   | IntAdd: s:seq a -> ss:(seq (seq a)){length ss = p} -> prf: interleave #a #p s ss 
                     -> x:a -> i:nat{i < p} 
                     -> interleave #a #p (append1 s x) (append1seq #a ss x i)     
-
-#push-options "--print_universes --print_implicits"
 
 (* map every element of the interleaved sequence to its source *)
 val interleave_map (#a:eqtype) 
@@ -65,3 +152,5 @@ type all_sorted (#a:eqtype) (lte: a -> a -> bool) (ss: seq (seq a)) =
 val merge_interleave (#a:eqtype) (lte: a -> a -> bool) 
                      (ss: seq (seq a) {all_sorted #a lte ss /\ length ss > 0}):
   s:seq a {interleave #a #(length ss) s ss /\ sorted #a lte s} 
+*)
+
